
\documentclass{article}
\usepackage{amsmath,amssymb,amsthm,latexsym,paralist,relsize}
\usepackage{graphicx}
\usepackage[margin=1.5in]{geometry}
\usepackage{titling}
\usepackage{xcolor}
\usepackage{float}
\usepackage{enumitem}
\usepackage{caption}
\usepackage{subcaption}
\setlength{\droptitle}{-10em}   % This is your set screw
\DeclareRobustCommand{\stirling}{\genfrac\{\}{0pt}{}}
\theoremstyle{definition}

%\newtheorem{definition}{Definition}
%\newtheorem{proof}{Proof}
%\newtheorem{remark}{Remark}


\newtheorem{problem}{Problem}
\newtheorem*{solution}{Solution}
\newtheorem*{resources}{Resources}


% Self Explanatory
\newtheorem{theorem}{Theorem}[section]
\newtheorem{definition}{Definition}
\newtheorem{corollary}{Corollary}[theorem]

\newtheorem{example}{Example}

\newtheorem{lemma}[theorem]{Lemma}


\newcommand{\ep}{\varepsilon}
\newcommand{\vp}{\varphi}
\newcommand{\lam}{\lambda}
\newcommand{\Lam}{\Lambda}
%\newcommand{\abs}[1]{\ensuremath{\left\lvert#1\right\rvert}} % This clashes with the physics package
%\newcommand{\norm}[1]{\ensuremath{\left\lVert#1\right\rVert}} % This clashes with the physics package

\newcommand{\floor}[1]{\ensuremath{\left\lfloor#1\right\rfloor}}
\newcommand{\ceil}[1]{\ensuremath{\left\lceil#1\right\rceil}}
\newcommand{\A}{\mathbb{A}}
\newcommand{\B}{\mathbb{B}}
\newcommand{\C}{\mathbb{C}}
\newcommand{\D}{\mathbb{D}}
\newcommand{\E}{\mathbb{E}}
\newcommand{\F}{\mathbb{F}}
\newcommand{\K}{\mathbb{K}}
\newcommand{\N}{\mathbb{N}}
\newcommand{\Q}{\mathbb{Q}}
\newcommand{\R}{\mathbb{R}}
\newcommand{\T}{\mathbb{T}}
\newcommand{\X}{\mathbb{X}}
\newcommand{\Y}{\mathbb{Y}}
\newcommand{\Z}{\mathbb{Z}}
\newcommand{\As}{\mathcal{A}}
\newcommand{\Bs}{\mathcal{B}}
\newcommand{\Cs}{\mathcal{C}}
\newcommand{\Ds}{\mathcal{D}}
\newcommand{\Es}{\mathcal{E}}
\newcommand{\Fs}{\mathcal{F}}
\newcommand{\Gs}{\mathcal{G}}
\newcommand{\Hs}{\mathcal{H}}
\newcommand{\Is}{\mathcal{I}}
\newcommand{\Js}{\mathcal{J}}
\newcommand{\Ks}{\mathcal{K}}
\newcommand{\Ls}{\mathcal{L}}
\newcommand{\Ms}{\mathcal{M}}
\newcommand{\Ns}{\mathcal{N}}
\newcommand{\Os}{\mathcal{O}}
\newcommand{\Ps}{\mathcal{P}}
\newcommand{\Qs}{\mathcal{Q}}
\newcommand{\Rs}{\mathcal{R}}
\newcommand{\Ss}{\mathcal{S}}
\newcommand{\Ts}{\mathcal{T}}
\newcommand{\Us}{\mathcal{U}}
\newcommand{\Vs}{\mathcal{V}}
\newcommand{\Ws}{\mathcal{W}}
\newcommand{\Xs}{\mathcal{X}}
\newcommand{\Ys}{\mathcal{Y}}
\newcommand{\Zs}{\mathcal{Z}}
\newcommand{\ab}{\textbf{a}}
\newcommand{\bb}{\textbf{b}}
\newcommand{\cb}{\textbf{c}}
\newcommand{\db}{\textbf{d}}
\newcommand{\ub}{\textbf{u}}
%\renewcommand{\vb}{\textbf{v}} % This clashes with the physics package (the physics package already defines the \vb command)
\newcommand{\wb}{\textbf{w}}
\newcommand{\xb}{\textbf{x}}
\newcommand{\yb}{\textbf{y}}
\newcommand{\zb}{\textbf{z}}
\newcommand{\Ab}{\textbf{A}}
\newcommand{\Bb}{\textbf{B}}
\newcommand{\Cb}{\textbf{C}}
\newcommand{\Db}{\textbf{D}}
\newcommand{\eb}{\textbf{e}}
\newcommand{\ex}{\textbf{e}_x}
\newcommand{\ey}{\textbf{e}_y}
\newcommand{\ez}{\textbf{e}_z}
\newcommand{\abar}{\overline{a}}
\newcommand{\bbar}{\overline{b}}
\newcommand{\cbar}{\overline{c}}
\newcommand{\dbar}{\overline{d}}
\newcommand{\ubar}{\overline{u}}
\newcommand{\vbar}{\overline{v}}
\newcommand{\wbar}{\overline{w}}
\newcommand{\xbar}{\overline{x}}
\newcommand{\ybar}{\overline{y}}
\newcommand{\zbar}{\overline{z}}
\newcommand{\Abar}{\overline{A}}
\newcommand{\Bbar}{\overline{B}}
\newcommand{\Cbar}{\overline{C}}
\newcommand{\Dbar}{\overline{D}}
\newcommand{\Ubar}{\overline{U}}
\newcommand{\Vbar}{\overline{V}}
\newcommand{\Wbar}{\overline{W}}
\newcommand{\Xbar}{\overline{X}}
% \newcommand{\ybar}{\overline{y}}
\newcommand{\Zbar}{\overline{Z}}
\newcommand{\Aint}{A^\circ}
\newcommand{\Bint}{B^\circ}
\newcommand{\limk}{\lim_{k\to\infty}}
\newcommand{\limm}{\lim_{m\to\infty}}
\newcommand{\limn}{\lim_{n\to\infty}}
\newcommand{\limx}[1][a]{\lim_{x\to#1}}
\newcommand{\liminfm}{\liminf_{m\to\infty}}
\newcommand{\limsupm}{\limsup_{m\to\infty}}
\newcommand{\liminfn}{\liminf_{n\to\infty}}
\newcommand{\limsupn}{\limsup_{n\to\infty}}
\newcommand{\sumkn}{\sum_{k=1}^n}
\newcommand{\sumin}{\sum_{i=1}^n}
\newcommand{\sumk}[1][1]{\sum_{k=#1}^\infty}
\newcommand{\summ}[1][1]{\sum_{m=#1}^\infty}
\newcommand{\sumn}[1][1]{\sum_{n=#1}^\infty}
\newcommand{\emp}{\varnothing}
\newcommand{\exc}{\backslash}
\newcommand{\sub}{\subseteq}
\newcommand{\sups}{\supseteq}
\newcommand{\capp}{\bigcap}
\newcommand{\cupp}{\bigcup}
\newcommand{\kupp}{\bigsqcup}
\newcommand{\cappkn}{\bigcap_{k=1}^n}
\newcommand{\cuppkn}{\bigcup_{k=1}^n}
\newcommand{\kuppkn}{\bigsqcup_{k=1}^n}
\newcommand{\cappk}[1][1]{\bigcap_{k=#1}^\infty}
\newcommand{\cuppk}[1][1]{\bigcup_{k=#1}^\infty}
\newcommand{\cappm}[1][1]{\bigcap_{m=#1}^\infty}
\newcommand{\cuppm}[1][1]{\bigcup_{m=#1}^\infty}
\newcommand{\cappn}[1][1]{\bigcap_{n=#1}^\infty}
\newcommand{\cuppn}[1][1]{\bigcup_{n=#1}^\infty}
\newcommand{\kuppk}[1][1]{\bigsqcup_{k=#1}^\infty}
\newcommand{\kuppm}[1][1]{\bigsqcup_{m=#1}^\infty}
\newcommand{\kuppn}[1][1]{\bigsqcup_{n=#1}^\infty}
\newcommand{\cappa}{\bigcap_{\alpha\in I}}
\newcommand{\cuppa}{\bigcup_{\alpha\in I}}
\newcommand{\kuppa}{\bigsqcup_{\alpha\in I}}
\newcommand{\Rx}{\overline{\mathbb{R}}}
\newcommand{\dx}{\,dx}
\newcommand{\dy}{\,dy}
\newcommand{\dt}{\,dt}
\newcommand{\dax}{\,d\alpha(x)}
\newcommand{\dbx}{\,d\beta(x)}
\DeclareMathOperator{\glb}{\text{glb}}
\DeclareMathOperator{\lub}{\text{lub}}
\newcommand{\xh}{\widehat{x}}
\newcommand{\yh}{\widehat{y}}
\newcommand{\zh}{\widehat{z}}
\newcommand{\<}{\langle}
\renewcommand{\>}{\rangle}
\renewcommand{\iff}{\Leftrightarrow}
\DeclareMathOperator{\im}{\text{im}}
\let\spn\relax\let\Re\relax\let\Im\relax
\DeclareMathOperator{\spn}{\text{span}}
\DeclareMathOperator{\Re}{\text{Re}}
\DeclareMathOperator{\Im}{\text{Im}}
\DeclareMathOperator{\diag}{\text{diag}}

\newcommand{\RN}[1]{%
  \textup{\uppercase\expandafter{\romannumeral#1}}%
}

\newcommand\defeq{\mathrel{\overset{\makebox[0pt]{\mbox{\normalfont\tiny\sffamily def}}}{=}}}

\newcommand{\bhat}{\hat{\beta_1}}

% Typed name, course, email address
\title{CSCE 420 : HW 3}
\author{William Allen}
\date{\today}

\begin{document}
\maketitle

\textbf{I did the last homework in Word and had a mental breakdown as a consequence. I'm doing this in latex this time just as God intended.}
\begin{enumerate}[label=\textbf{\arabic*.}]
  %% MAJOR PROBLEM  
  \item Translate the following sentences into First-Order Logic. Remember to break things down to simple concepts (with short predicate and function names), and make use of quantifiers. For example, “tasteDelicious(someRedTomatos)”, is not broken down enough; instead we would be looking for a formulation such as: 

    “$\exists x$ tomato(x)$\land$red(x)$\land$taste(x,delicious)”. 

    See the lecture slides for more examples and guidance.
    \begin{enumerate}
      \item bowling balls are sporting equipment
      \item all domesticated horses have an owner
      \item the rider of a horse can be different than the owner
      \item horses move faster than frogs
      \item a finger is any digit on a hand other than the thumb
      \item an isosceles triangle is defined as a polygon with 3 edges, which are connected at 3 vertices, where 2 (but not 3) edges have the same length 
    \end{enumerate}
    
    %% SOLUTION
    \vspace{1em} 
    \textit{ Sol. }
    \vspace{1em}
    \begin{quote}
      \begin{enumerate}
        \item $\forall x\;\text{ball}(x) \land \text{heavy}(x) \land \text{hasThreeHoles}(x) \rightarrow \text{sportingEquipment}(x)$
        \item $\forall x\;\text{horse}(x) \land \text{domesticated}(x) \rightarrow \exists y\;\text{ownerOf}(x,y)$
        \item $\forall x\;\text{horse}(x) \land \exists y\;\text{riderOf}(x,y) \land \exists z\;\text{ownerOf}(x,z) \rightarrow y \neq z$
        \item $\forall x\;\text{horse}(x) \land \forall y\;\text{frog}(y) \rightarrow \text{movesFaster}(x,y)$
        \item $\forall x\;\text{digit}(x) \land \text{onHand}(x) \land \text{notThumb}(x) \rightarrow \text{finger}(x)$
        \item $\forall x\;\text{isoscelesTriangle}(x) \iff \text{polygon}(x) \land \text{hasEdges}(x,3) \land \text{hasVertices}(x,3) \land \exists a,b,c\;\text{lengthOf}(a,b,x) \land \text{lengthOf}(b,c,x) \land \text{lengthOf}(a,c,x) \land (\text{equals}(a,b) \lor \text{equals}(b,c) \lor \text{equals}(a,c)) \land \neg(\text{equals}(a,b) \land \text{equals}(b,c) \land \text{equals}(a,c))$
     \end{enumerate} 
    \end{quote}

    \newpage
  
  %% MAJOR PROBLEM
  \item Convert the following first-order logic sentence into CNF:
  \begin{equation*}
    \forall x\;\text{person}(x) \land [\exists z \;\text{petOf}(x,z) \land \forall y \; \text{petOf}(x,y) \rightarrow \text{dog}(y)] \rightarrow \text{doglover}(x)
  \end{equation*}
  %% SOLUTION
  \vspace{1em} 
  \textit{ Sol. }
  \begin{quote}
    Remove implications
    \begin{equation*}
    \forall x\; [\lnot \text{person}(x) \lor (\lnot \exists z \;\text{petOf}(x,z) \lor \lnot \forall y \; \text{petOf}(x,y) \lor \text{dog}(y)) \lor \text{doglover}(x)]
    \end{equation*}

    Move $\lnot$ inwards:
    \begin{equation*}
    \forall x\; [\lnot \text{person}(x) \lor ( \forall z \;\lnot\text{petOf}(x,z) \lor  \exists y \; \lnot\text{petOf}(x,y) \lor \text{dog}(y)) \lor \text{doglover}(x)]
    \end{equation*}

    Skolemization (removing existential quantifiers):
    \begin{equation*}
      \forall x\; [\lnot \text{person}(x) \lor (\forall z \;\lnot \text{petOf}(x, z) \lor \lnot\text{petOf}(x, g(x)) \lor \text{dog}(g(x))) \lor \text{doglover}(x)]
    \end{equation*}

    Drop universal quantifiers:
    \begin{equation*}
      \lnot \text{person}(x) \lor (\lnot \text{petOf}(x, z) \lor \lnot\text{petOf}(x, g(x)) \lor \text{dog}(g(x))) \lor \text{doglover}(x)
    \end{equation*}

    No distribution required, we are done.

  \end{quote}
  
  \newpage

  \item Determine whether or not the following pairs of predicates are unifiable. If they are, give the
  most-general unifier and show the result of applying the substitution to each predicate. If they are
  not unifiable, indicate why. Capital letters represent variables; constants and function names are
  lowercase. For example, ‘loves(A,hay)’ and ‘loves(horse,hay)’ are unifiable, the unifier is
  u={A/horse}, and the unified expression is ‘loves(horse,hay)’ for both.
  \begin{enumerate}
    \item owes(owner(X), citibank, cost(X)), owes(owner(ferrari), Z, cost(Y))
    \item gives(bill, jerry, book21), gives(X, brother(X),Z)
    \item opened(X, result(open(X),s0))), opened(toolbox, Z)
  \end{enumerate}

  %% SOLUTION
  \vspace{1em} 
  \textit{ Sol. }
  \begin{quote}
  \begin{enumerate}
    \item The most general unifier is \{X/ferrari, Z/citibank, Y/cost(ferrari)\}. After applying the substitution, the predicates become:\newline
      owes(owner(ferrari), citibank, cost(ferrari))
    \item The predicates are not unifiable. The second predicate states that X gives something to brother(X). This implies that brother(X) refers to X's sibling, and therefore, X cannot simultaneously refer to bill and jerry. Hence, the predicates cannot be unified.
    \item The most general unifier is \{X/toolbox, Z/result(open(toolbox),s0)\}. After applying the substitution, the predicates become:\newline
      opened(toolbox, result(open(toolbox),s0))
  \end{enumerate}
  \end{quote}
  \newpage

  \item Consider the following situation:\newline

  \textit{
    Marcus is a Pompeian.\\
    All Pompeians are Romans.\\
    Ceasar is a ruler.\\
    All Romans are either loyal to Caesar or hate Caesar (but not both).\\
    Everyone is loyal to someone.\\
    People only try to assassinate rulers they are not loyal to.\\
    Marcus tries to assassinate Caesar.\\
  }
  \begin{enumerate}
    \item Translate these sentences to First-Order Logic.
    \item Prove that Marcus hates Caesar using Natural Deduction. In the same style as the examples in the lecture slides, label all derived sentences with the ROI used, which prior sentences were used, and what unifier was used.
    \item Convert all the sentences to CNF
    \item Prove that Marcus hates Ceasar using Resolution Refutation
  \end{enumerate}
  
  %% SOLUTION
  \vspace{1em} 
  \textit{ Sol. }
  \begin{quote}
  \begin{enumerate}
    \item 

      \begin{enumerate}
        \item $\forall x(\text{Pompeian}(x) \rightarrow \text{Roman}(x))$
        \item $\text{Ruler}(Ceasar)$
        \item $\forall x(\text{Roman}(x) \rightarrow ((\text{Loyal}(x,Ceasar) \land \neg \text{Hate}(x,Ceasar)) \lor(\text{Hate}(x,Ceasar) \land \neg \text{Loyal}(x,Ceasar))))$
        \item $\forall x \exists y(\text{Loyal}(x,y))$
        \item $\forall x \forall y((\text{Ruler}(y) \land \neg \text{Loyal}(x,y)) \rightarrow \text{Assassinate}(x,y))$
        \item $\text{Pompeian}(Marcus)$
        \item $\text{Assassinate}(Marcus,Ceasar)$
      \end{enumerate}
      \vspace{0.5em}
    \item

      \begin{enumerate}[label=\arabic*.]
        \item $\forall x(\text{Pompeian}(x) \rightarrow \text{Roman}(x))$ (Premise)
        \item $\text{Ruler}(Ceasar)$ (Premise)
        \item $\forall x(\text{Roman}(x) \rightarrow ((\text{Loyal}(x,Ceasar) \land \neg \text{Hate}(x,Ceasar)) \lor(\text{Hate}(x,Ceasar) \land \neg \text{Loyal}(x,Ceasar))))$ (Premise)
        \item $\forall x \forall y((\text{Ruler}(y) \land \neg \text{Loyal}(x,y)) \rightarrow \text{Assassinate}(x,y))$ (Premise)
        \item $\text{Pompeian}(Marcus)$ (Premise)
        \item $\text{Assassinate}(Marcus,Ceasar)$ (Premise)
        \item $\text{Roman}(Marcus)$ (Modus Ponens of 1 and 5 using substitution $x/Marcus$)
        \item $(\text{Loyal}(Marcus,Ceasar) \land \neg \text{Hate}(Marcus,Ceasar)) \lor(\text{Hate}(Marcus,Ceasar) \land \neg \text{Loyal}(Marcus,Ceasar))$ (Modus Ponens of 3 and 7 using substitution $x/Marcus$)
        \item $\neg \text{Loyal}(Marcus, Ceasar) \land \text{Ruler}(Ceasar)$ (Modus Tollens of 4 and 6 using substitution $x/Marcus$, $y/Ceasar$)
        \item $\neg \text{Loyal}(Marcus, Ceasar)$ (Simplification of 9)
        \item $\text{Hate}(Marcus,Ceasar) \land \neg \text{Loyal}(Marcus,Ceasar)$ (Disjunctive Syllogism of 8 and 10)
        \item $\text{Hate}(Marcus,Ceasar)$ (Simplification of 11)
    \end{enumerate}

  \item 
    \begin{enumerate}
    \item $\neg\text{Pompeian}(x) \lor \text{Roman}(x)$
    \item $\text{Ruler}(Ceasar)$
    \item $(\neg\text{Roman}(x) \land \neg\text{Roman}(x)) \lor (\neg\text{Roman}(x) \land \text{Loyal}(x,Ceasar)) \lor (\neg\text{Roman}(x) \land \text{Hate}(x,Ceasar)) \lor (\neg\text{Hate}(x,Ceasar) \land \text{Loyal}(x,Ceasar)) \lor (\neg\text{Hate}(x,Ceasar) \land \text{Hate}(x,Ceasar))$
    \item $\text{Loyal}(x,f(x))$
    \item $\neg\text{Ruler}(y) \lor \text{Loyal}(x,y) \lor \text{Assassinate}(x,y)$
    \item $\text{Pompeian}(Marcus)$
    \item $\text{Assassinate}(Marcus,Ceasar)$
    \end{enumerate}
\end{enumerate}

\end{quote}
\newpage
\item Write a KB in First-Order Logic with rules/axioms for:
  \begin{enumerate}
    \item Map-coloring – every state must be exactly 1 color, and adjacent states must be different
colors. Assume possible colors are states are defined using unary predicate like color(red)
or state(WA). To say a state has a color, use a binary predicate, e.g. ‘color(WA,red)’.
    \item Sammy’s Sport Shop – include sentences for specific facts like obs(1,W) or label(2,B),
as well as for general constraints about the boxes and colors. Use binary predicate
‘contains(x,q)’ to represent that box x contains tennis balls of color q (where q could be
W, Y, or B).
    \item Wumpus World - Write rules for which rooms are ‘stenchy’, ‘breezy’, and ‘safe’. (hint:
define a helper concept called ‘adjacent(x,y,p,q)’ which defines when a room at
coordinates (x,y) is adjacent to another room at (p,q), and x,y,p,q are integers 1-4.
    \item 4-Queens – assume row(1)…row(4) and col(1)…col(4) are facts; write rules that
describe configurations of 4 queens such that none can attack each other, using
‘queen(r,c)’ to represent that there is a queen in row r and col c.
  \end{enumerate}

  %% SOLUTION
  \vspace{1em} 
  \textit{ Sol. }
  \begin{quote}
  \begin{enumerate}
    \item 

      \begin{enumerate}
        \item adjacent(WA, NT) $\lor$ adjacent(WA, SA) $\lor$ adjacent(NT, Q) $\lor$ adjacent(SA, Q) $\lor$ adjacent(SA, NSW)  $\lor$ adjacent(SA, V) $\lor$ adjacent(Q, NSW) $\lor$ adjacent(V, NSW)
        \item $\forall x \; \forall y \; \forall z$ (adjacent(x,y) $\land$ color(x,z) $\rightarrow \lnot$ color(y,z))
        \item $\forall x \; \exists y \;$ color(x,y)
      \end{enumerate}
      \vspace{0.5em}
    \item

      \begin{enumerate}
\item $\forall x \; (\text{label}(x, \text{W}) \rightarrow \lnot \text{contains}(x, \text{W}))$
\item $\forall x \; (\text{label}(x, \text{Y}) \rightarrow \lnot \text{contains}(x, \text{Y}))$
\item $\forall x \; (\text{label}(x, \text{B}) \rightarrow \lnot \text{contains}(x, \text{B}))$
\item $\forall x \; (\text{contains}(x, \text{W}) \rightarrow \lnot \text{contains}(x, \text{Y}))$
\item $\forall x \; (\text{contains}(x, \text{Y}) \rightarrow \lnot \text{contains}(x, \text{W}))$
\item $\forall x \; (\text{contains}(x, \text{B}) \rightarrow (\text{contains}(x, \text{W}) \land \text{contains}(x, \text{Y})))$
\item $\forall x \; (\text{obs}(x, \text{W}) \rightarrow (\text{contains}(x, \text{W}) \lor \text{contains}(x, \text{B})))$
\item $\forall x \; (\text{obs}(x, \text{Y}) \rightarrow (\text{contains}(x, \text{Y}) \lor \text{contains}(x, \text{B})))$
\item $\exists x \; \exists y \; \exists z \; (\text{contains}(x, \text{W}) \land \text{contains}(y, \text{Y}) \land \text{contains}(z, \text{B}) \land (x \neq y) \land (x \neq z) \land (y \neq z))$
      \end{enumerate}
      \vspace{0.5em}

    \item 
      \begin{enumerate}
        \item $adjacent(x,y,a,b) \leftrightarrow (x=a \land (y=b+1 \lor y=b-1)) \lor (y=b \land (x=a+1 \lor x=a-1))$
        \item $stench(x,y) \leftrightarrow \exists a,b(adjacent(x,y,a,b) \land wumpus(a,b))$
        \item $breeze(x,y) \leftrightarrow \exists a,b(adjacent(x,y,a,b) \land pit(a,b))$
        \item $safe(x,y) \leftrightarrow \lnot stench(x,y) \land \lnot breeze(x,y)$
      \end{enumerate}
      \vspace{0.5em}

  \item 
      \begin{enumerate}
        \item $row(1) \land row(2) \land row(3) \land row(4)$
        \item $col(1) \land col(2) \land col(3) \land col(4)$
        \item $\forall x(queen(x,1) \to \lnot \exists y(queen(y,1) \land y \neq x))$
        \item $\forall x(queen(x,2) \to \lnot \exists y(queen(y,2) \land y \neq x))$
        \item $\forall x(queen(x,3) \to \lnot \exists y(queen(y,3) \land y \neq x))$
        \item $\forall x(queen(x,4) \to \lnot \exists y(queen(y,4) \land y \neq x))$
        \item $\forall x\forall y\forall a\forall b((queen(x,y) \land queen(a,b)) \to (x \neq a \land y \neq b \land x+y \neq a+b \land x-y \neq a-b))$      
      \end{enumerate}
      \vspace{0.5em}
\end{enumerate}

\end{quote}

\end{enumerate}

\end{document}

